progress on refl/trans proof

examples/pseudo_bool/npbcScript.sml
@@ -2000,6 +2000,673 @@ Proof
   metis_tac[]
 QED
 
+(* NOTE: terminology & we fix the unchanged vars or the changed vars?
+  A formula fml can be extended over variables vars if
+  every assignment can be extended (maintaining its values on vars)
+  such that fml is satisfied *)
+Definition the_spec_def:
+  the_spec fml auxs w w' ⇔
+  (∀x. x ∉ auxs ⇒ w x = w' x) ∧
+  satisfies w' fml
+End
+
+Definition is_spec_def:
+  is_spec fml auxs ⇔
+  ∀w. ∃w'. the_spec fml auxs w w'
+End
+
+(* Syntactic representation of a partial order
+  to be used in dominance-with-auxiliaries:
+  ((f, g, us, vs, as), xs)
+  such that:
+  - |us| = |vs|
+  - all lists of variables us, vs, as (mutually) distinct
+  - vars(f) = us ∪ vs ∪ as
+  - vars(g) = us ∪ vs ∪ as
+  - |xs| = |us|
+*)
+Type aspo = ``: (npbc list # npbc list # var list # var list # var list) # var list``
+
+(* w ≤ w' iff
+  consider the assignment mapping
+    us -> w (xs)
+    vs -> w' (xs)
+    _  -> F
+  since g is a specification, there is an extension
+  of this mapping to all auxiliaries.
+  this extension satisfies f
+*)
+Definition po_of_aspo_def:
+  po_of_aspo (((f,g,us,vs,as),xs):aspo) =
+  λw w'.
+  let ss = ALOOKUP
+    (ZIP (us,MAP (INL o w) xs) ++
+     ZIP (vs,MAP (INL o w') xs)) in
+  let ww = assign ss (λn. F) in
+  ∃aww.
+    the_spec (set g) (set as) ww aww ∧
+    satisfies aww (set f)
+End
+
+Theorem finite_support_po_of_aspo:
+  finite_support (po_of_aspo (fuv,xs)) (set xs)
+Proof
+  PairCases_on`fuv`>>
+  rw[finite_support_def,po_of_aspo_def]>>
+  Cases_on`(∀x. MEM x xs ⇒ (w x ⇔ w' x))`>>simp[]>>
+  ho_match_mp_tac ConseqConvTheory.exists_eq_thm>>
+  rw[]>>
+  qmatch_goalsub_abbrev_tac`the_spec _ _ (assign ww _) _ ∧ _ ⇔ the_spec _ _ (assign ww' _) _ ∧ _`>>
+  qsuff_tac`ww = ww'`>>simp[]>>
+  unabbrev_all_tac>>
+  simp[o_DEF,MAP_MEM_BOOL]
+QED
+
+Definition good_aord_def:
+  good_aord (f,g,us,vs,as) ⇔
+  npbf_vars (set f) ⊆ set us ∪ set vs ∪ set as ∧
+  npbf_vars (set g) ⊆ set us ∪ set vs ∪ set as ∧
+  LENGTH us = LENGTH vs ∧
+  ALL_DISTINCT (us ++ vs ++ as) ∧
+  is_spec (set g) (set as)
+End
+
+Theorem LIST_REL_ALOOKUP:
+  LIST_REL R xs ys ∧
+  ALOOKUP (ZIP (xs,ys)) x = SOME y ⇒
+  R x y
+Proof
+  rw[LIST_REL_EVERY_ZIP]>>
+  drule ALOOKUP_MEM>>
+  gvs[EVERY_MEM,UNCURRY]>>
+  metis_tac[FST,SND]
+QED
+
+Theorem assign_ALOOKUP_skip:
+  LIST_REL (λu v. w u = w v) us vs ⇒
+  assign (ALOOKUP (ZIP (vs,MAP (INR ∘ Pos) us))) w n = w n
+Proof
+  rw[FUN_EQ_THM,assign_def]>>
+  drule LIST_REL_LENGTH>>
+  simp[ALOOKUP_ZIP_MAP_SND]>>
+  rename1`w n`>>
+  Cases_on`ALOOKUP (ZIP (vs,us)) n`>>
+  rw[]>>
+  drule_at Any LIST_REL_ALOOKUP>>
+  disch_then ho_match_mp_tac>>
+  irule EVERY2_sym>>
+  first_x_assum (irule_at Any)>>
+  simp[]
+QED
+
+Theorem reflexive_po_of_aspo:
+  good_aord (f,g,us,vs,as) ∧
+  LENGTH xs = LENGTH us ⇒
+  (set g) ⇂
+    ALOOKUP
+    (ZIP (vs,MAP (INR o Pos) us))
+  ⊨
+  (set f) ⇂
+    ALOOKUP
+    (ZIP (vs,MAP (INR o Pos) us)) ⇒
+  reflexive (po_of_aspo ((f,g,us,vs,as),xs))
+Proof
+  rw[reflexive_def,po_of_aspo_def,sat_implies_def]>>
+  fs[satisfies_subst_thm,good_aord_def]>>
+  gvs[is_spec_def]>>
+  qmatch_goalsub_abbrev_tac`the_spec _ _ w`>>
+  last_x_assum(qspec_then `w` assume_tac)>>
+  gvs[]>>
+  first_assum (irule_at Any)>>
+  gvs[the_spec_def]>>
+  rename1`satisfies w' (set f)`>>
+  `∀n. n ∈ set us ∪ set vs ∪ set as ⇒
+    (w' n ⇔ assign (ALOOKUP (ZIP (vs,MAP (INR ∘ Pos) us))) w' n)` by (
+    rw[]>>
+    simp[assign_def,ALOOKUP_ZIP_MAP_SND]
+    >- (
+      DEP_REWRITE_TAC[IMP_ALOOKUP_NONE]>>
+      fs[ALL_DISTINCT_APPEND])
+    >- (
+      Cases_on`ALOOKUP (ZIP (vs,us)) n`
+      >- gs[MAP_ZIP,ALOOKUP_NONE]>>
+      rename1`ALOOKUP _ _ = SOME yy`>>
+      `MEM yy us` by (
+        drule ALOOKUP_MEM>>
+        rw[MEM_ZIP,MEM_EL]>>
+        metis_tac[])>>
+      gvs[ALL_DISTINCT_APPEND,Abbr`w`]>>
+      simp[assign_def,ALOOKUP_ZIP_MAP_SND,ALOOKUP_APPEND]>>
+      Cases_on`ALOOKUP (ZIP (us,xs)) yy`
+      >- gs[MAP_ZIP,ALOOKUP_NONE]>>
+      simp[]>>
+      Cases_on`ALOOKUP (ZIP (vs,xs)) n`
+      >- gs[MAP_ZIP,ALOOKUP_NONE]>>
+      simp[]>>
+      DEP_REWRITE_TAC[IMP_ALOOKUP_NONE]>>
+      fs[ALL_DISTINCT_APPEND]>>
+      CONJ_TAC>- metis_tac[]>>
+      simp[]>>
+      gvs[MEM_EL]>>
+      rpt (qpat_x_assum`ALOOKUP _ _ = SOME _` mp_tac)>>
+      DEP_REWRITE_TAC [ALOOKUP_ALL_DISTINCT_EL_IMP]>>
+      simp[]>>rw[]>>
+      metis_tac[ALL_DISTINCT_EL_IMP])
+    >- (
+      DEP_REWRITE_TAC[IMP_ALOOKUP_NONE]>>
+      fs[ALL_DISTINCT_APPEND]>>
+      metis_tac[]))>>
+  first_x_assum(qspec_then`w'` mp_tac)>>
+  impl_tac >- (
+    qpat_x_assum`satisfies w' _` mp_tac>>
+    match_mp_tac (GEN_ALL npbf_vars_satisfies)>>
+    asm_exists_tac>>
+    metis_tac[])>>
+  match_mp_tac (GEN_ALL npbf_vars_satisfies)>>
+  asm_exists_tac>>
+  metis_tac[]
+QED
+
+Theorem ALOOKUP_ZIP_same:
+  ∀ls.
+  ALOOKUP (ZIP (ls,ls)) n = if MEM n ls then SOME n else NONE
+Proof
+  Induct>>rw[]>>gvs[]
+QED
+
+Theorem transitive_po_of_aspo:
+  good_aord (f,g,us,vs,as) ∧
+  LENGTH xs = LENGTH us ∧
+  LENGTH ws = LENGTH us ∧
+  LENGTH bs = LENGTH as ∧
+  LENGTH cs = LENGTH as ∧
+  ALL_DISTINCT (ws ++ bs ++ cs) ∧
+  (∀y. MEM y ws ⇒ ¬ MEM y us ∧ ¬ MEM y vs ∧ ¬ MEM y as) ∧
+  (∀y. MEM y bs ⇒ ¬ MEM y us ∧ ¬ MEM y vs ∧ ¬ MEM y as) ∧
+  (∀y. MEM y cs ⇒ ¬ MEM y us ∧ ¬ MEM y vs ∧ ¬ MEM y as)
+  ⇒
+  set g ∪
+  (set g) ⇂
+    ALOOKUP
+    (ZIP (us,MAP (INR o Pos) vs) ++
+     ZIP (vs,MAP (INR o Pos) ws) ++
+     ZIP (as,MAP (INR o Pos) bs)) ∪
+  (set g) ⇂
+    ALOOKUP
+     (ZIP (vs,MAP (INR o Pos) ws) ++
+      ZIP (as,MAP (INR o Pos) cs)) ∪
+  (set f) ∪
+  (set f) ⇂
+    ALOOKUP
+    (ZIP (us,MAP (INR o Pos) vs) ++
+     ZIP (vs,MAP (INR o Pos) ws) ++
+     ZIP (as,MAP (INR o Pos) bs))
+  ⊨
+  (set f) ⇂
+    ALOOKUP
+     (ZIP (vs,MAP (INR o Pos) ws) ++
+      ZIP (as,MAP (INR o Pos) cs)) ⇒
+  transitive (po_of_aspo ((f,g,us,vs,as),xs))
+Proof
+  rw[transitive_def,po_of_aspo_def,sat_implies_def]>>
+  fs[satisfies_subst_thm]>>
+  fs[good_aord_def,ALL_DISTINCT_APPEND,is_spec_def]>>
+  (* pick extension for the goal *)
+  qmatch_goalsub_abbrev_tac`the_spec _ _ w`>>
+  last_x_assum(qspec_then `w` mp_tac)>>
+  strip_tac>>
+  fs[Abbr`w`]>>
+  first_assum (irule_at Any)>>
+  rename1`the_spec _ _ _ g3`>>
+  pop_assum mp_tac>>
+  rename1`the_spec _ _ _ g2`>>
+  ntac 2 (pop_assum mp_tac)>>
+  rename1`the_spec _ _ _ g1`>>
+  ntac 3 strip_tac>>
+  (* Construct the massive assignment to all variables *)
+  qabbrev_tac`
+    ww =
+    assign
+      (ALOOKUP
+         (ZIP (us,MAP (INL ∘ x) xs) ++
+          ZIP (vs,MAP (INL ∘ y) xs) ++
+          ZIP (ws,MAP (INL ∘ z) xs) ++
+          ZIP (as,MAP (INL ∘ g1) as) ++
+          ZIP (bs,MAP (INL ∘ g2) as) ++
+          ZIP (cs,MAP (INL ∘ g3) as)
+      ))
+      (λn. F)`>>
+  gvs[the_spec_def]>>
+  `∀n. n ∈ set us ∪ set vs ∪ set as ⇒ (g1 n ⇔ ww n)` by (
+    rw[]>>
+    simp[Abbr`ww`,assign_def,ALOOKUP_ZIP_MAP_SND,ALOOKUP_APPEND]
+    >- (
+      Cases_on`ALOOKUP (ZIP (us,xs)) n`
+      >- gs[MAP_ZIP,ALOOKUP_NONE]>>
+      simp[])
+    >- (
+      Cases_on`ALOOKUP (ZIP (vs,xs)) n`
+      >- gs[MAP_ZIP,ALOOKUP_NONE]>>
+      DEP_REWRITE_TAC[IMP_ALOOKUP_NONE]>>
+      rw[]>>
+      metis_tac[])
+    >- (
+      simp[ALOOKUP_ZIP_same]>>
+      DEP_REWRITE_TAC[IMP_ALOOKUP_NONE]>>
+      simp[]>>
+      metis_tac[]))>>
+  `∀n. n ∈ set us ∪ set vs ∪ set as ⇒ (
+    g2 n ⇔
+    assign
+    (ALOOKUP
+      (ZIP (us,MAP (INR ∘ Pos) vs) ++
+       ZIP (vs,MAP (INR ∘ Pos) ws) ++
+       ZIP (as,MAP (INR ∘ Pos) bs))) ww n)` by (
+    rw[]>>
+    simp[Abbr`ww`,assign_def,ALOOKUP_ZIP_MAP_SND,ALOOKUP_APPEND]
+    >- (
+      Cases_on`ALOOKUP (ZIP (us,xs)) n`
+      >- gs[MAP_ZIP,ALOOKUP_NONE]>>
+      Cases_on`ALOOKUP (ZIP (us,vs)) n`
+      >- gs[MAP_ZIP,ALOOKUP_NONE]>>
+      simp[]>>
+      rename1`ALOOKUP _ yy`>>
+      `MEM yy vs` by (
+        drule ALOOKUP_MEM>>
+        rw[MEM_ZIP,MEM_EL]>>
+        metis_tac[])>>
+      Cases_on`ALOOKUP (ZIP (vs,xs)) yy`
+      >- gs[MAP_ZIP,ALOOKUP_NONE]>>
+      DEP_REWRITE_TAC[IMP_ALOOKUP_NONE]>>
+      CONJ_TAC>- metis_tac[]>>
+      simp[]>>
+      qpat_x_assum`MEM n us` mp_tac>>
+      qpat_x_assum`MEM yy vs` mp_tac>>
+      rw[MEM_EL]>>gvs[]>>
+      rpt (qpat_x_assum`ALOOKUP _ _ = SOME _` mp_tac)>>
+      DEP_REWRITE_TAC [ALOOKUP_ALL_DISTINCT_EL_IMP]>>
+      simp[]>>rw[]>>
+      metis_tac[ALL_DISTINCT_EL_IMP])
+    >- (
+      Cases_on`ALOOKUP (ZIP (vs,xs)) n`
+      >- gs[MAP_ZIP,ALOOKUP_NONE]>>
+      Cases_on`ALOOKUP (ZIP (vs,ws)) n`
+      >- gs[MAP_ZIP,ALOOKUP_NONE]>>
+      simp[]>>
+      rename1`ALOOKUP _ _ = SOME yy`>>
+      `MEM yy ws` by (
+        drule ALOOKUP_MEM>>
+        rw[MEM_ZIP,MEM_EL]>>
+        metis_tac[])>>
+      Cases_on`ALOOKUP (ZIP (ws,xs)) yy`
+      >- gs[MAP_ZIP,ALOOKUP_NONE]>>
+      simp[]>>
+      ntac 4 (
+        DEP_ONCE_REWRITE_TAC[IMP_ALOOKUP_NONE]>>
+        CONJ_TAC>- metis_tac[]>>
+        simp[])>>
+      qpat_x_assum`MEM n vs` mp_tac>>
+      qpat_x_assum`MEM yy ws` mp_tac>>
+      rw[MEM_EL]>>gvs[]>>
+      rpt (qpat_x_assum`ALOOKUP _ _ = SOME _` mp_tac)>>
+      DEP_REWRITE_TAC [ALOOKUP_ALL_DISTINCT_EL_IMP]>>
+      simp[]>>rw[]>>
+      metis_tac[ALL_DISTINCT_EL_IMP])
+    >- (
+      Cases_on`ALOOKUP (ZIP (as,bs)) n`
+      >- gs[MAP_ZIP,ALOOKUP_NONE]>>
+      rename1`ALOOKUP _ _ = SOME yy`>>
+      `MEM yy bs` by (
+        drule ALOOKUP_MEM>>
+        rw[MEM_ZIP,MEM_EL]>>
+        metis_tac[])>>
+      ntac 6 (
+        DEP_ONCE_REWRITE_TAC[IMP_ALOOKUP_NONE]>>
+        CONJ_TAC>- metis_tac[]>>
+        simp[])>>
+      Cases_on`ALOOKUP (ZIP (bs,as)) yy`
+      >- gs[MAP_ZIP,ALOOKUP_NONE]>>
+      simp[]>>
+      qpat_x_assum`MEM n as` mp_tac>>
+      qpat_x_assum`MEM yy bs` mp_tac>>
+      rw[MEM_EL]>>gvs[]>>
+      rpt (qpat_x_assum`ALOOKUP _ _ = SOME _` mp_tac)>>
+      DEP_REWRITE_TAC [ALOOKUP_ALL_DISTINCT_EL_IMP]>>
+      simp[]>>rw[]>>
+      metis_tac[ALL_DISTINCT_EL_IMP]))>>
+  `∀n. n ∈ set us ∪ set vs ∪ set as ⇒ (
+    g3 n ⇔
+    assign
+    (ALOOKUP
+      (ZIP (vs,MAP (INR ∘ Pos) ws) ++
+       ZIP (as,MAP (INR ∘ Pos) cs))) ww n)` by (
+    rw[]>>
+    simp[Abbr`ww`,assign_def,ALOOKUP_ZIP_MAP_SND,ALOOKUP_APPEND]
+    >- (
+      Cases_on`ALOOKUP (ZIP (us,xs)) n`
+      >- gs[MAP_ZIP,ALOOKUP_NONE]>>
+      simp[]>>
+      DEP_REWRITE_TAC[IMP_ALOOKUP_NONE]>>
+      CONJ_TAC>- metis_tac[]>>
+      simp[])
+    >- (
+      Cases_on`ALOOKUP (ZIP (vs,xs)) n`
+      >- gs[MAP_ZIP,ALOOKUP_NONE]>>
+      Cases_on`ALOOKUP (ZIP (vs,ws)) n`
+      >- gs[MAP_ZIP,ALOOKUP_NONE]>>
+      simp[]>>
+      rename1`ALOOKUP _ _ = SOME yy`>>
+      `MEM yy ws` by (
+        drule ALOOKUP_MEM>>
+        rw[MEM_ZIP,MEM_EL]>>
+        metis_tac[])>>
+      Cases_on`ALOOKUP (ZIP (ws,xs)) yy`
+      >- gs[MAP_ZIP,ALOOKUP_NONE]>>
+      simp[]>>
+      ntac 3 (
+        DEP_ONCE_REWRITE_TAC[IMP_ALOOKUP_NONE]>>
+        CONJ_TAC>- metis_tac[]>>
+        simp[])>>
+      qpat_x_assum`MEM n vs` mp_tac>>
+      qpat_x_assum`MEM yy ws` mp_tac>>
+      rw[MEM_EL]>>gvs[]>>
+      rpt (qpat_x_assum`ALOOKUP _ _ = SOME _` mp_tac)>>
+      DEP_REWRITE_TAC [ALOOKUP_ALL_DISTINCT_EL_IMP]>>
+      simp[]>>rw[]>>
+      metis_tac[ALL_DISTINCT_EL_IMP])
+    >- (
+      Cases_on`ALOOKUP (ZIP (as,cs)) n`
+      >- gs[MAP_ZIP,ALOOKUP_NONE]>>
+      rename1`ALOOKUP _ _ = SOME yy`>>
+      `MEM yy cs` by (
+        drule ALOOKUP_MEM>>
+        rw[MEM_ZIP,MEM_EL]>>
+        metis_tac[])>>
+      ntac 6 (
+        DEP_ONCE_REWRITE_TAC[IMP_ALOOKUP_NONE]>>
+        CONJ_TAC>- metis_tac[]>>
+        simp[])>>
+      Cases_on`ALOOKUP (ZIP (cs,as)) yy`
+      >- gs[MAP_ZIP,ALOOKUP_NONE]>>
+      simp[]>>
+      qpat_x_assum`MEM n as` mp_tac>>
+      qpat_x_assum`MEM yy cs` mp_tac>>
+      rw[MEM_EL]>>gvs[]>>
+      rpt (qpat_x_assum`ALOOKUP _ _ = SOME _` mp_tac)>>
+      DEP_REWRITE_TAC [ALOOKUP_ALL_DISTINCT_EL_IMP]>>
+      simp[]>>rw[]>>
+      metis_tac[ALL_DISTINCT_EL_IMP]))>>
+  first_x_assum(qspec_then`ww` mp_tac)>>
+  impl_tac >- (
+    rw[]>>
+    metis_tac[GEN_ALL npbf_vars_satisfies])>>
+  metis_tac[GEN_ALL npbf_vars_satisfies]
+QED
+
+Theorem imp_sat_ord_po_of_spo:
+  good_ord (f,us,vs) ∧
+  LENGTH xs = LENGTH us ∧
+  fml ∪ {not c} ⊨
+  (set f) ⇂
+  (λn.
+    case ALOOKUP (ZIP (us,xs)) n of
+      SOME v =>
+        (case w v of NONE => SOME (INR (Pos v)) | r => r)
+    | NONE => ALOOKUP (ZIP (vs, MAP (INR o Pos) xs)) n) ⇒
+  sat_ord (fml ∪ {not c}) (po_of_spo ((f,us,vs),xs)) w
+Proof
+  rw[sat_ord_def,po_of_spo_def]>>
+  gvs[sat_implies_def]>>
+  first_x_assum drule>>
+  fs[good_ord_def,ALL_DISTINCT_APPEND]>>
+  simp[satisfies_subst_thm]>>
+  match_mp_tac (GEN_ALL npbf_vars_satisfies)>>
+  asm_exists_tac>>rw[]>>
+  simp[assign_def,ALOOKUP_ZIP_MAP_SND,ALOOKUP_APPEND]
+  >- (
+    Cases_on`ALOOKUP (ZIP (us,xs)) n`
+    >- gs[MAP_ZIP,ALOOKUP_NONE]>>
+    DEP_REWRITE_TAC[IMP_ALOOKUP_NONE]>>
+    CONJ_TAC>- metis_tac[]>>
+    simp[assign_def]>>
+    Cases_on`w x`>>simp[])
+  >- (
+    Cases_on`ALOOKUP (ZIP (vs,xs)) n`
+    >- gs[MAP_ZIP,ALOOKUP_NONE]>>
+    DEP_REWRITE_TAC[IMP_ALOOKUP_NONE]>>
+    CONJ_TAC>- metis_tac[]>>
+    simp[assign_def])
+QED
+
+Theorem imp_sat_strict_ord_po_of_spo:
+  good_ord (f,us,vs) ∧
+  LENGTH xs = LENGTH us ∧
+  fml ∪ {not c} ⊨
+  (set f) ⇂
+  (λn.
+    case ALOOKUP (ZIP (us,xs)) n of
+      SOME v =>
+        (case w v of NONE => SOME (INR (Pos v)) | r => r)
+    | NONE => ALOOKUP (ZIP (vs, MAP (INR o Pos) xs)) n) ∧
+  unsatisfiable (
+    fml ∪ {not c} ∪
+    (set f) ⇂
+    (λn.
+      case ALOOKUP (ZIP (vs,xs)) n of
+        SOME v =>
+          (case w v of NONE => SOME (INR (Pos v)) | r => r)
+      | NONE => ALOOKUP (ZIP (us, MAP (INR o Pos) xs)) n)) ⇒
+  sat_strict_ord (fml ∪ {not c}) (po_of_spo ((f,us,vs),xs)) w
+Proof
+  rw[sat_strict_ord_def]
+  >-
+    metis_tac[imp_sat_ord_po_of_spo]>>
+  CCONTR_TAC>>
+  qpat_x_assum`unsatisfiable _` mp_tac>>
+  simp[unsatisfiable_def,satisfiable_def]>>
+  asm_exists_tac>>
+  fs[po_of_spo_def]>>
+  qpat_x_assum`_ ⊨ _` kall_tac>>
+  fs[good_ord_def,ALL_DISTINCT_APPEND]>>
+  pop_assum mp_tac>>
+  simp[satisfies_subst_thm]>>
+  match_mp_tac (GEN_ALL npbf_vars_satisfies)>>
+  asm_exists_tac>>rw[]>>
+  simp[assign_def,ALOOKUP_ZIP_MAP_SND,ALOOKUP_APPEND]
+  >- (
+    Cases_on`ALOOKUP (ZIP (us,xs)) n`
+    >- gs[MAP_ZIP,ALOOKUP_NONE]>>
+    DEP_REWRITE_TAC[IMP_ALOOKUP_NONE]>>
+    CONJ_TAC>- metis_tac[]>>
+    simp[])
+  >- (
+    Cases_on`ALOOKUP (ZIP (vs,xs)) n`
+    >- gs[MAP_ZIP,ALOOKUP_NONE]>>
+    DEP_REWRITE_TAC[IMP_ALOOKUP_NONE]>>
+    CONJ_TAC>- metis_tac[]>>
+    simp[assign_def]>>
+    Cases_on`w x`>>simp[])
+QED
+
+Definition sat_obj_po_def:
+  sat_obj_po pres spoopt fopt s t ⇔
+  ∀w.
+    satisfies w s ⇒
+    ∃w'.
+      (∀x. x ∈ pres ⇒ w x = w' x) ∧
+      satisfies w' t ∧
+      OPTION_ALL (λspo. (po_of_spo spo) w' w) spoopt ∧
+      eval_obj fopt w' ≤ eval_obj fopt w
+End
+
+Definition redundant_wrt_obj_po_def:
+  redundant_wrt_obj_po f pres ord obj c ⇔
+    sat_obj_po pres ord obj f (f ∪ {c})
+End
+
+Definition list_list_insert_def:
+  list_list_insert [] ys = LN ∧
+  list_list_insert xs [] = LN ∧
+  list_list_insert (x::xs) (y::ys) = insert x y (list_list_insert xs ys)
+End
+
+Theorem lookup_list_list_insert:
+  ∀xs ys. lookup n (list_list_insert xs ys) = ALOOKUP (ZIP(xs,ys)) n
+Proof
+  Induct_on ‘xs’ \\ Cases_on ‘ys’ \\ fs [list_list_insert_def,ZIP_def]
+  \\ rw [lookup_insert]
+QED
+
+(* The substituted order formula used in dominance order *)
+Definition dom_subst_def:
+  (dom_subst w NONE = []) ∧
+  (dom_subst w (SOME ((f,us,vs),xs)) =
+  let us_xs = list_list_insert us xs in
+  let vs_xs = list_list_insert vs xs in
+  let ww = (λn.
+    case lookup n us_xs of
+      SOME v =>
+        (case w v of NONE => SOME (INR (Pos v)) | r => r)
+    | NONE =>
+        (case lookup n vs_xs of
+         | SOME v => SOME (INR (Pos v))
+         | NONE => NONE)) in
+  MAP (subst ww) f)
+End
+
+(* Any installed spo must satisfy these conditions *)
+Definition good_spo_def:
+  good_spo spo ⇔
+  good_ord (FST spo) ∧
+  reflexive (po_of_spo spo) ∧
+  transitive (po_of_spo spo) ∧
+  LENGTH (SND spo) = LENGTH (FST (SND (FST spo)))
+End
+
+Theorem ALOOKUP_ZIP_MAP:
+  ∀xs ys f n.
+    ALOOKUP (ZIP (xs,MAP f ys)) n =
+    case ALOOKUP (ZIP (xs,ys)) n of
+    | NONE => NONE
+    | SOME v => SOME (f v)
+Proof
+  Induct \\ Cases_on ‘ys’ \\ gvs [ZIP_def] \\ rw []
+QED
+
+Theorem substitution_redundancy_obj_po:
+  OPTION_ALL good_spo ord ∧
+  (∀x. x ∈ pres ⇒ w x = NONE) ∧
+  f ∪ {not c} ⊨ ((f ∪ {c}) ⇂ w ∪
+    (case obj of NONE => {}
+      | SOME obj => {obj_constraint w obj})) ∧
+  f ∪ {not c} ⊨ set (dom_subst w ord)
+  ⇒
+  redundant_wrt_obj_po f pres ord obj c
+Proof
+  simp[Once sat_implies_def]
+  \\ rw[redundant_wrt_obj_po_def, sat_obj_po_def,not_thm]
+  \\ rename1`satisfies s f`
+  \\ Cases_on ‘satisfies_npbc s c’
+  >- (
+    qexists_tac`s`>>simp[]>>
+    Cases_on`ord`>>
+    fs[good_spo_def]>>
+    metis_tac[reflexive_def,reflexive_po_of_spo,PAIR])
+  \\ first_x_assum drule_all
+  \\ rw [subst_thm]
+  \\ first_x_assum $ irule_at Any
+  \\ rw[]
+  >-
+    gvs[assign_def]
+  >-
+    fs[eval_obj_def,satisfies_def,PULL_EXISTS,subst_thm]
+  >- (
+    Cases_on`ord`>>fs[good_spo_def]>>
+    PairCases_on`x`>>fs[]>>
+    drule imp_sat_ord_po_of_spo>>
+    disch_then drule>>
+    fs[dom_subst_def,LIST_TO_SET_MAP,lookup_list_list_insert,ALOOKUP_ZIP_MAP]>>
+    disch_then drule>>
+    simp[sat_ord_def]>>
+    disch_then match_mp_tac>>
+    fs[not_thm])
+  >- (
+    every_case_tac
+    >- fs [eval_obj_def] >>
+    fs [satisfies_def,PULL_EXISTS,subst_thm,satisfies_npbc_obj_constraint])
+QED
+
+Theorem good_spo_dominance:
+  good_spo ((f,us,vs),xs) ∧
+  (∀x. x ∈ pres ⇒ w x = NONE) ∧
+  C ⊆ fml ∧
+  (∀w.
+    satisfies w C ⇒
+    ∃w'.
+      (∀x. x ∈ pres ⇒ w x = w' x) ∧
+      satisfies w' fml ∧
+      po_of_spo ((f,us,vs),xs) w' w ∧
+      eval_obj obj w' ≤ eval_obj obj w) ∧
+  fml ∪ {not c} ⊨ C ⇂ w ∧
+  fml ∪ {not c} ⊨
+  (set f) ⇂
+    (λn.
+      case ALOOKUP (ZIP (us,xs)) n of
+        SOME v =>
+          (case w v of NONE => SOME (INR (Pos v)) | r => r)
+      | NONE => ALOOKUP (ZIP (vs, MAP (INR o Pos) xs)) n) ∧
+  unsatisfiable (
+    fml ∪ {not c} ∪
+    (set f) ⇂
+    (λn.
+      case ALOOKUP (ZIP (vs,xs)) n of
+        SOME v =>
+          (case w v of NONE => SOME (INR (Pos v)) | r => r)
+      | NONE => ALOOKUP (ZIP (us, MAP (INR o Pos) xs)) n)) ∧
+  (case obj of
+    NONE => T
+  | SOME obj =>
+    fml ∪ {not c} ⊨ {obj_constraint w obj}) ⇒
+  (∀w.
+    satisfies w C ⇒
+    ∃w'.
+      (∀x. x ∈ pres ⇒ w x = w' x) ∧
+      satisfies_npbc w' c ∧
+      satisfies w' fml ∧
+      po_of_spo ((f,us,vs),xs) w' w ∧
+      eval_obj obj w' ≤ eval_obj obj w)
+Proof
+  rw[]>>
+  `conf_valid' C (fml DIFF C) pres (po_of_spo ((f,us,vs),xs)) obj` by (
+    fs[conf_valid'_def]>>rw[]>>
+    last_x_assum drule>>
+    rw[]>>
+    pop_assum (irule_at Any)>>
+    fs[satisfies_def,SUBSET_DEF])>>
+  imp_res_tac dominance_conf_valid>>
+  pop_assum mp_tac>>
+  `C ∪ (fml DIFF C) = fml` by (
+    fs[EXTENSION,SUBSET_DEF]>>
+    metis_tac[])>>
+  simp[]>>
+  disch_then drule>>
+  disch_then (qspec_then`set xs` mp_tac)>>
+  simp[finite_support_po_of_spo]>>
+  impl_tac>- (
+    fs[good_spo_def]>>
+    match_mp_tac imp_sat_strict_ord_po_of_spo>>
+    simp[])>>
+  simp[conf_valid'_def,redundant_wrt_obj_po_def,sat_obj_po_def]>>
+  rw[]>>
+  pop_assum drule>>
+  rw[]>>
+  pop_assum (irule_at Any)>>
+  fs[satisfies_def]>>
+  metis_tac[]
+QED
+
+
+
 Definition sem_concl_def:
   (sem_concl fml obj NoConcl = T) ∧
   (sem_concl fml obj DSat = satisfiable fml) ∧
@@ -2099,5 +2766,10 @@ Definition weaken_spt_def:
   | SOME c =>
     (delete v l, n-Num(ABS c))
 End
+
+
+
+
+
 
 val _ = export_theory();
